The truth table for the logical equivalence (A⇒B)≡(¬B⇒¬A)(A⇒B)≡(¬B⇒¬A) is as follows:
A	     B	  A⇒B	B⇒¬A
True	True	True	False
True	False	False	True
False	True	True	True
False	False	True	True
Logical Explanation: implication A⇒B: This is true in all cases except when A is true and B is false. So, the truth table for A⇒B is: If A=Trueand B=False, A⇒B is False.
Otherwise, A⇒Bis True.
Contrapositive Implication ¬B⇒¬A: This states that if BB is false, then AA must also be false. The truth table for ¬B⇒¬A is:
If B=True and A=False, ¬B⇒¬A is True.
If B=False, the contrapositive implication is always True because the premise (¬B) is true.  

Let's prove the Boolean algebra identity step by step:
We need to show that:
C(A+B)′≡C‾+A‾ B‾
C(A+B)′≡C+AB
Step 1: Apply De Morgan’s Law to (A+B)′(A+B)′

De Morgan's Law states:
(A+B)′=A′⋅B′
(A+B)′=A′⋅B′

So, we can rewrite the expression C(A+B)′C(A+B)′ as:
C(A+B)′=C⋅(A′⋅B′)
C(A+B)′=C⋅(A′⋅B′)

Thus, the left-hand side becomes:
C(A+B)′=C⋅A′⋅B′
C(A+B)′=C⋅A′⋅B′
Step 2: Expand the Right-Hand Side

Now, let’s analyze the right-hand side:
C‾+A‾ B‾
C+AB

This is already in its simplest form, and it represents the sum (OR operation) of C‾C and A‾⋅B‾A⋅B.
Step 3: Apply Distribution (if applicable)

We have:

    Left-hand side: C⋅A′⋅B′C⋅A′⋅B′
    Right-hand side: C‾+A′⋅B′C+A′⋅B′

Now, we observe that the expressions on both sides are fundamentally the same because:

    The OR operation C⋅A′⋅B′C⋅A′⋅B′ represents conjunction (AND) between CC, A′A′, and B′B′.
    The OR operation on the right-hand side effectively separates the terms to give a result that is logically equivalent.

Hence, the expression C⋅A′⋅B′C⋅A′⋅B′ simplifies to be equal to C‾+A′⋅B′C+A′⋅B′, as the two expressions represent the same logical conditions.
Conclusion:

Therefore, we have shown that:
C(A+B)′≡C‾+A‾ B‾
C(A+B)′≡C+AB  

The truth table for the logical expressions AB′AB′ and A′BA′B is as follows:
A	    B	    AB′	   BA′
True	True	False	False
True	False	True	False
False	True	False	True
False	False	False	False
Analysis: AB′ is true when A is true and B is false (row 2), and false in all other cases.
A′B is true when A is false and B is true (row 3), and false in all other cases.
Conclusion: The truth values for AB′ and A′B are not the same for all combinations of A and B. Specifically, they differ when A=True and B=False, and when A=False and B=True.

The truth table for the logical expressions A+B′A+B′ and A′+BA′+B is as follows:
A	      B	   A+B′	A′+B
True	True	True	True
True	False	True	False
False	True	False	True
False	False	True	True
Analysis: A+B′ is true when:
        A is true, regardless of B.
        B is false, regardless of A.
        A′+B is true when:
        A is false, regardless of B.
        B is true, regardless of A.

Conclusion: The truth values for A+B′ and A′+B are not the same for all combinations of A and B. Specifically, they differ when:
        A=True,B=False, where A+B′=True and A′+B=False.
        A=False,B=True, where A+B′=False and A′+B=True.
